BlockCacheSystem/BlockSystem.i.dfy
@@ -1537,58 +1537,58 @@ module BlockSystem {
 
   lemma NewRequestReadNodeDoesntOverlap(k: Constants, s: Variables, s': Variables, dop: DiskOp, vop: VOp, step: M.Step, id: D.ReqId)
   requires Inv(k, s)
-  requires Machine(k, s, s', dop, vop, step)
+  requires M.NextStep(k.machine, s.machine, s'.machine, dop, vop, step)
   requires dop.ReqReadNodeOp?
   requires id in s.disk.reqWriteNodes
   ensures !overlap(dop.loc, s.disk.reqWriteNodes[id])
   {
-    MachineStepPreservesInv(k, s, s', dop, vop, step);
+    /*MachineStepPreservesInv(k, s, s', dop, vop, step);
     assert !overlap(
         s'.disk.reqReadNodes[dop.id],
         s'.disk.reqWriteNodes[id]);
-    assert !overlap(dop.loc, s'.disk.reqWriteNodes[id]);
+    assert !overlap(dop.loc, s'.disk.reqWriteNodes[id]);*/
   }
 
   lemma NewRequestReadIndirectionTableDoesntOverlap(k: Constants, s: Variables, s': Variables, dop: DiskOp, vop: VOp, step: M.Step, id: D.ReqId)
   requires Inv(k, s)
-  requires Machine(k, s, s', dop, vop, step)
+  requires M.NextStep(k.machine, s.machine, s'.machine, dop, vop, step)
   requires dop.ReqReadIndirectionTableOp?
   requires id in s.disk.reqWriteIndirectionTables
   ensures !overlap(dop.loc, s.disk.reqWriteIndirectionTables[id])
   {
-    MachineStepPreservesInv(k, s, s', dop, vop, step);
+    /*MachineStepPreservesInv(k, s, s', dop, vop, step);
     assert !overlap(
         s'.disk.reqReadIndirectionTables[dop.id],
         s'.disk.reqWriteIndirectionTables[id]);
-    assert !overlap(dop.loc, s'.disk.reqWriteIndirectionTables[id]);
+    assert !overlap(dop.loc, s'.disk.reqWriteIndirectionTables[id]);*/
   }
 
   lemma NewRequestWriteNodeDoesntOverlap(k: Constants, s: Variables, s': Variables, dop: DiskOp, vop: VOp, step: M.Step, id: D.ReqId)
   requires Inv(k, s)
-  requires Machine(k, s, s', dop, vop, step)
+  requires M.NextStep(k.machine, s.machine, s'.machine, dop, vop, step)
   requires dop.ReqWriteNodeOp?
   requires id in s.disk.reqWriteNodes
   ensures !overlap(dop.reqWriteNode.loc, s.disk.reqWriteNodes[id])
   {
-    MachineStepPreservesInv(k, s, s', dop, vop, step);
+    /*MachineStepPreservesInv(k, s, s', dop, vop, step);
     assert !overlap(
         s'.disk.reqWriteNodes[dop.id],
         s'.disk.reqWriteNodes[id]);
-    assert !overlap(dop.reqWriteNode.loc, s'.disk.reqWriteNodes[id]);
+    assert !overlap(dop.reqWriteNode.loc, s'.disk.reqWriteNodes[id]);*/
   }
 
   lemma NewRequestWriteIndirectionTableDoesntOverlap(k: Constants, s: Variables, s': Variables, dop: DiskOp, vop: VOp, step: M.Step, id: D.ReqId)
   requires Inv(k, s)
-  requires Machine(k, s, s', dop, vop, step)
+  requires M.NextStep(k.machine, s.machine, s'.machine, dop, vop, step)
   requires dop.ReqWriteIndirectionTableOp?
   requires id in s.disk.reqWriteIndirectionTables
   ensures !overlap(dop.reqWriteNode.loc, s.disk.reqWriteIndirectionTables[id])
   {
-    MachineStepPreservesInv(k, s, s', dop, vop, step);
+    /*MachineStepPreservesInv(k, s, s', dop, vop, step);
     assert !overlap(
         s'.disk.reqWriteIndirectionTables[dop.id],
         s'.disk.reqWriteIndirectionTables[id]);
-    assert !overlap(dop.reqWriteNode.loc, s'.disk.reqWriteIndirectionTables[id]);
+    assert !overlap(dop.reqWriteNode.loc, s'.disk.reqWriteIndirectionTables[id]);*/
   }
 
 }
